[Checkpoint] Modify Hoare triple notation to make it compatible with oracle refinement.

src/Layer1/HoareLogic.v
@@ -7,30 +7,47 @@ Set Implicit Arguments.
 Definition precond := oracle -> @pred addr addr_dec (set value).
 Definition postcond {T: Type} := T -> @pred addr addr_dec (set value).
 Definition crashcond := @pred addr addr_dec (set value).
+Definition augpostcond {T: Type} := oracle -> disk (set value) -> T -> @pred addr addr_dec (set value).
+Definition augcrashcond := oracle -> disk (set value) -> @pred addr addr_dec (set value).
 
-
-Definition hoare_triple {T: Type} (pre: precond) (p: prog T) (post: @postcond T) (crash: crashcond):=
-  forall o d,
+Definition hoare_triple {T: Type} (pre: precond) (p: prog T) (post: @postcond T) (crash: crashcond) (augpost: augpostcond) (augcrash: augcrashcond):=
+  fun o d =>
     pre o d ->
     (exists ret,
         exec o d p ret /\
         ((exists d' r,
              ret = Finished d' r
-             /\ post r d') \/
+             /\ post r d' /\ augpost o d r d') \/
          (exists d',
-             ret = Crashed d' /\ crash d')))%type.
+             ret = Crashed d' /\ crash d' /\ augcrash o d d')))%type.
 
 
   
 Notation
-  "<< o >> pre p << r >> post crash" :=
+  "<< o , d >> pre p << r >> post crash" :=
   (forall F, hoare_triple
           (fun o d => (F * pre * [[ oracle_ok p o d ]]) d)%pred
           p%pred
           (fun r => F * post)%pred
-          (F * crash)%pred)
-    (at level 10, o at next level, pre at next level, p at next level, r at next level, post at next level, crash at next level,
-     format "'[v' '[  ' '<<' o '>>' '//' '[' pre ']' '//' '[' p ']' ']' '//' '[  ' '<<' r '>>' '//' '[' post ']' '//' '[' crash ']' ']' ']'").
+          (F * crash)%pred
+          (fun _ _ _ => any)
+          (fun _ _ => any)
+          o d)      
+    (at level 10, o at next level, d at next level, pre at next level, p at next level, r at next level, post at next level, crash at next level,
+     format "'[v' '[  ' '<<' o ','  d '>>' '//' '[' pre ']' '//' '[' p ']' ']' '//' '[  ' '<<' r '>>' '//' '[' post ']' '//' '[' crash ']' ']' ']'").
+
+Notation
+  "<< o , d >> pre p << r >> post crash augpost augcrash" :=
+  (forall F, hoare_triple
+          (fun o d => (F * pre * [[ oracle_ok p o d ]]) d)%pred
+          p%pred
+          (fun r => F * post)%pred
+          (F * crash)%pred
+          (fun o d r => F * augpost)%pred
+          (fun o d => F * augcrash)%pred
+          o d)      
+    (at level 10, o at next level, d at next level, pre at next level, p at next level, r at next level, post at next level, crash at next level, augpost at next level, augcrash at next level,
+     format "'[v' '[  ' '<<' o ','  d '>>' '//' '[' pre ']' '//' '[' p ']' ']' '//' '[  ' '<<' r '>>' '//' '[' post ']' '//' '[' crash ']' '//' '[' augpost ']' '//' '[' augcrash ']' ']' ']'").
 
 (*
 Notation
@@ -44,6 +61,7 @@ Notation
      format "'[v' '{{' e1 '}}' '//' '[  ' '<<' o '>>' '//' pre '//' p ']' '//' '[  ' '<<' r '>>' '//' post '//' crash ']' ']'").
 *)
 
+(*
 Theorem hoare_triple_strengthen_pre:
   forall T (p: prog T) (pre pre': precond) post crash,
   hoare_triple pre p post crash ->
@@ -55,7 +73,6 @@ Proof.
   eapply H0; eauto.
 Qed.
 
-(*
 Theorem hoare_triple_weaken_post_weak:
   forall T (p: prog T) pre (post post': postcond) crash,
   hoare_triple pre p post crash ->
@@ -170,10 +187,10 @@ Qed.
 *)
 
 Theorem hoare_triple_equivalence :
-  forall T (p p': prog T) pre post crash,
-    hoare_triple pre p post crash ->
+  forall T (p p': prog T) o d pre post crash ap ac,
+    hoare_triple pre p post crash ap ac o d ->
     prog_equiv p p' ->
-    hoare_triple pre p' post crash.
+    hoare_triple pre p' post crash ap ac o d.
 Proof.
   unfold hoare_triple; intros.
   edestruct H; eauto; cleanup.
@@ -183,6 +200,30 @@ Proof.
   end.
 Qed.
 
+Theorem remember_oracle_ok :
+  forall T (p: prog T) o d pre post crash ap ac,
+    (oracle_ok p o d ->
+  << o, d >>
+   pre
+   p
+  << r >>
+   (post r)
+   crash
+   (ap o d r)
+   (ac o d)) ->
+  << o, d >>
+   pre
+   p
+  << r >>
+   (post r)
+   crash
+   (ap o d r)
+   (ac o d).
+Proof.
+  unfold hoare_triple; intros.
+  eapply H; eauto.
+  destruct_lift  H0; eauto.
+Qed.
 
 Ltac monad_simpl_one :=
   match goal with
@@ -194,40 +235,43 @@ Ltac monad_simpl_one :=
 Ltac monad_simpl := repeat monad_simpl_one.
 
 Theorem bind_ok:
-  forall T T' (p1: prog T) (p2: T -> prog T') pre1 post1 crash1 pre2 post2 crash2 pre3 post3 crash3,
-  << o >>
+  forall T T' (p1: prog T) (p2: T -> prog T') pre1 post1 crash1 pre2 post2 crash2 pre3 post3 crash3 o d,
+  (forall o1,
+   (exists o2, o = o1++o2) ->      
+   << o1, d >>
    pre1
    p1
   << r >>
    (post1 r)
-   crash1 ->
+   crash1) ->
   ( pre3 =p=> pre1 ) ->
-  (forall F d r,
+  (forall F r,
       (F * pre1)%pred d ->
       post1 r =p=> pre2) ->
-  (forall F d1 d2 r1 r2,
-      (F * pre1)%pred d1 ->
+  (forall F d2 r1 r2,
+      (F * pre1)%pred d ->
       (F * post1 r1)%pred d2 ->
       (F * pre2)%pred d2 ->
       post2 r2 =p=> post3 r2) ->
-  (forall F d,
+  (forall F,
       (F * pre1)%pred d ->
       crash1 =p=> crash3) ->
-  (forall F d1 d2 r1,
-      (F * pre1)%pred d1 ->
+  (forall F d2 r1,
+      (F * pre1)%pred d ->
       (F * post1 r1)%pred d2 ->
       (F * pre2)%pred d2 ->
       crash2 =p=> crash3) ->
-  (forall F d d' r,
+  (forall F o2 d2 r,
       (F * pre1)%pred d ->
-      (F * post1 r)%pred d' ->
-      << o >>
+      (F * post1 r)%pred d2 ->
+      (exists o1, o = o1++o2) ->   
+      << o2, d2 >>
          pre2
          (p2 r)
        << r >>
        (post2 r)
        crash2) ->
-  << o >>
+  << o, d >>
      pre3
      (Bind p1 p2)
   << r >>
@@ -266,21 +310,21 @@ Proof.
     rewrite app_nil_r.
     eexists; split; intuition eauto.
     right; eexists; intuition eauto.
-    pred_apply; cancel.
+    pred_apply' H12; cancel.
     eauto.
 Qed.
 
 
 Theorem crash_weaken:
-  forall T (p: prog T) pre post crash1 crash2,
-  << o >>
+  forall T (p: prog T) pre post crash1 crash2 o d,
+  << o, d >>
    pre
    p
   << r >>
    (post r)
    crash1 ->
   (crash1 =p=> crash2) ->
-  << o >>
+  << o, d >>
      pre
      p
   << r >>
@@ -293,20 +337,20 @@ Proof.
   split_ors; cleanup;
     eexists; intuition eauto.
   right; eexists; intuition eauto.
-  pred_apply; cancel; eauto.
+  clear H5; pred_apply; cancel; eauto.
 Qed.
 
 
 Theorem post_weaken:
-  forall T (p: prog T) pre post1 post2 crash,
-  << o >>
+  forall T (p: prog T) pre post1 post2 crash o d,
+  << o, d >>
    pre
    p
   << r >>
    (post1 r)
    crash  ->
   (forall r, post1 r =p=> post2 r) ->
-  << o >>
+  << o, d >>
      pre
      p
   << r >>
@@ -319,19 +363,19 @@ Proof.
   split_ors; cleanup;
     eexists; intuition eauto.
   left; do 2 eexists; intuition eauto.
-  pred_apply; cancel; eauto.
+  clear H5; pred_apply; cancel; eauto.
 Qed.
 
 Theorem pre_strengthen:
-  forall T (p: prog T) pre1 pre2 post crash,
-  << o >>
+  forall T (p: prog T) pre1 pre2 post crash o d,
+  << o, d >>
    pre1
    p
   << r >>
    (post r)
    crash ->
   (pre2 =p=> pre1) ->
-  << o >>
+  << o, d >>
      pre2
      p
   << r >>
@@ -343,16 +387,41 @@ Proof.
   pred_apply; cancel; eauto.
 Qed.
 
+Theorem pre_strengthen_aug:
+  forall T (p: prog T) pre1 pre2 post crash ap ac o d,
+  << o, d >>
+   pre1
+   p
+  << r >>
+   (post r)
+   crash
+   (ap o d r)
+   (ac o d) ->
+  (pre2 =p=> pre1) ->
+  << o, d >>
+     pre2
+     p
+  << r >>
+     (post r)
+     crash
+     (ap o d r)
+     (ac o d).
+Proof.
+  unfold hoare_triple; intros.
+  edestruct H; eauto.
+  pred_apply; cancel; eauto.
+Qed.
+
 
 Theorem add_frame:
-  forall T (p: prog T) pre post crash F,
-  << o >>
+  forall T (p: prog T) pre post crash F o d,
+  << o, d >>
    pre
    p
   << r >>
    (post r)
    crash  ->
-  << o >>
+  << o, d >>
      (F * pre)
      p
   << r >>
@@ -365,21 +434,21 @@ Proof.
   cleanup; split_ors; cleanup;
     eexists; intuition eauto.
   left; do 2 eexists; intuition eauto.
-  pred_apply; cancel; eauto.
+  clear H4; pred_apply; cancel; eauto.
   right; eexists; intuition eauto.
-  pred_apply; cancel; eauto.
+  clear H4; pred_apply; cancel; eauto.
 Qed.
 
 Theorem extract_exists:
-  forall T V (p: prog T) pre post crash,
+  forall T V (p: prog T) pre post crash o d,
     (forall (v:V),
-  << o >>
+  << o, d >>
    (pre v)
    p
   << r >>
    (post r)
    crash) ->
-  << o >>
+  << o, d >>
      (exists v, pre v)
      p
   << r >>
@@ -390,4 +459,170 @@ Proof.
   destruct_lifts.
   eapply H; eauto.
   pred_apply' H0; cancel; eauto.
+Qed.
+
+Theorem extract_exists_aug:
+  forall T V (p: prog T) pre post crash ap ac o d,
+    (forall (v:V),
+  << o, d >>
+   (pre v)
+   p
+  << r >>
+   (post r)
+   crash
+   (ap o d r)
+   (ac o d)) ->
+  << o, d >>
+     (exists v, pre v)
+     p
+  << r >>
+     (post r)
+     crash
+     (ap o d r)
+     (ac o d).
+Proof.
+  unfold hoare_triple; intros.
+  destruct_lifts.
+  eapply H; eauto.
+  pred_apply' H0; cancel; eauto.
+Qed.
+
+Theorem remove_augcons:
+  forall T (p: prog T) pre post crash (augpost: augpostcond) (augcrash: augcrashcond) o d,
+  << o, d >>
+   pre
+   p
+  << r >>
+   (post r)
+   crash ->
+  (forall F d' r,
+      (F * pre)%pred d ->
+      exec o d p (Finished d' r) ->
+      (F * post r)%pred d' ->
+      (F * augpost o d r)%pred d') ->
+  (forall F d',
+      (F * pre)%pred d ->
+      exec o d p (Crashed d') ->
+      (F * crash)%pred d' ->
+      (F * augcrash o d)%pred d') ->
+  << o, d >>
+     pre
+     p
+  << r >>
+     (post r)
+     crash
+     (augpost o d r)
+     (augcrash o d).
+Proof.
+  unfold hoare_triple; intros.
+  edestruct H; eauto; cleanup.
+  
+  split_ors; cleanup.
+  - 
+    eexists; split; intuition eauto.
+    left; do 2 eexists; intuition eauto.
+    eapply H0; eauto.
+    pred_apply; cancel.
+    
+  - 
+    eexists; split; intuition eauto.
+    right; eexists; intuition eauto.
+    eapply H1; eauto.
+    pred_apply; cancel.
+Qed.
+
+
+Theorem bind_ok_aug:
+  forall T T' (p1: prog T) (p2: T -> prog T') pre1 post1 crash1 pre2 post2 crash2 pre3 post3 crash3 augpost augcrash o d,
+  (forall o1,
+   (exists o2, o = o1++o2) ->
+   << o1, d >>
+   pre1
+   p1
+  << r >>
+   (post1 r)
+   crash1) ->
+  ( pre3 =p=> pre1 ) ->
+  (forall F r,
+      (F * pre1)%pred d ->
+      post1 r =p=> pre2) ->
+  (forall F d2 r1 r2,
+      (F * pre1)%pred d ->
+      (F * post1 r1)%pred d2 ->
+      (F * pre2)%pred d2 ->
+      post2 r2 =p=> post3 r2) ->
+  (forall F,
+      (F * pre1)%pred d ->
+      crash1 =p=> crash3) ->
+  (forall F d2 r1,
+      (F * pre1)%pred d ->
+      (F * post1 r1)%pred d2 ->
+      (F * pre2)%pred d2 ->
+      crash2 =p=> crash3) ->
+  (forall o1 o2 F d1 r1,
+      (F * pre1)%pred d ->
+      exec o1 d p1 (Finished d1 r1) ->
+      (F * post1 r1)%pred d1 ->
+      (o = o1++o2) ->
+      << o2, d1 >>
+         pre2
+         (p2 r1)
+       << r >>
+       (post2 r)
+       crash2
+       (augpost o d r)
+       (augcrash o d)
+       ) ->
+  (forall F o1 d',
+      (F * pre1)%pred d ->
+      exec o1 d p1 (Crashed d') ->
+      (F * crash1)%pred d' ->
+      (exists o2, o = o1++o2) ->
+      (F * augcrash o d)%pred d') ->
+  << o, d >>
+     pre3
+     (Bind p1 p2)
+  << r >>
+     (post3 r)
+     crash3
+     (augpost o d r)
+     (augcrash o d)
+     .
+Proof.
+  unfold hoare_triple; intros.
+  simpl in *; destruct_lifts; cleanup.
+  rewrite H0 in H7.
+  edestruct H; eauto.
+  pred_apply' H7; cancel; eauto.
+  
+  cleanup.
+  split_ors; cleanup.
+  - specialize H10 with (1:=H8).
+    edestruct H5; eauto.
+    pred_apply' H13; norm.
+    cancel.
+    erewrite H1; eauto; cancel.
+    intuition eauto.
+
+    cleanup.
+    split_ors; cleanup;
+      eexists; split; intuition eauto.
+
+    left; do 2 eexists; intuition eauto.
+    pred_apply' H16; cancel; eauto.
+    eapply H2; eauto.
+    erewrite <- H1; eauto.
+    
+    right; eexists; intuition eauto.
+    pred_apply' H16; cancel; eauto.
+    eapply H4; eauto.
+    erewrite <- H1; eauto.
+  - specialize H11 with (1:=H8); cleanup.
+    rewrite app_nil_r in *.
+    eexists; split; intuition eauto.
+    right; eexists; intuition eauto.
+    pred_apply' H13; cancel.
+    eauto.
+    eapply H6; eauto.
+    exists nil; rewrite app_nil_r; eauto.
 Qed.
