src/BlockAllocator/BlockAllocator.v
@@ -1,3 +1,2 @@
 Require Export BlockAllocator.Definitions.
 Require Export BlockAllocator.Facts.
-Require Export BlockAllocator.Specs.
